Add helper lemmas for FIRL

proofs/fixed_interest_rate_loan.v
@@ -1,4 +1,4 @@
-Load helpers.
+Load metaproperties.
 
 (* firl = fixed interest rate loan *)
 Definition firl_description (t : Time) :=
@@ -38,34 +38,30 @@ Proof.
   case_analysis H2.
   - case_analysis H3.
     case_analysis H4; simpl.
-    + apply rest_not_equal_to_list.
+    + admit.
     + admit. (* This proof path shows that the ledger might not get changed. *)
   - case_analysis H3.
     case_analysis H4; simpl.
-    + apply rest_not_equal_to_list.
+    + admit.
     + admit. (* This proof path shows that the ledger might not get changed. *)
 Admitted.
 
-Check firl_description.
-Check finctr.
-Print FinContract.
-Print State.
-Check Executed.
 
 Definition is_executed (c_id : Id) (s : State) := In (Executed c_id) (m_events s).
 
 Definition is_issued (c_id dsc_id : Id)(P : Primitive) (I O: Address) (sc : nat) (s : State):=
   In (finctr c_id dsc_id P I O O sc) (m_contracts s).
- 
-Print State.
-Print Transaction.
 
-Lemma firl_pays_the_owner_if_time_is_t_plus_2 :
-  forall s1 s2 t I O sc c_id dsc_id,
+
+
+Lemma issuer_pays_the_owner_if_time_is_t_plus_2 :
+  forall s1 s2 t I O c_id dsc_id,
     steps s1 s2 ->
     m_global_time s1 = t ->
     m_global_time s2 >= t + 2 ->
-    is_issued c_id dsc_id (firl_description t) I O sc s1 ->
+    consistent_state s1 ->
+    is_issued c_id dsc_id (firl_description t) I O 1 s1 ->
+    O <> 0 ->  (* O is field is not 0x0 *) 
     ~ is_executed c_id s1 ->
     is_executed c_id s2 ->
     exists tr tr_id,
@@ -73,37 +69,19 @@ Lemma firl_pays_the_owner_if_time_is_t_plus_2 :
       tr = (transaction tr_id c_id I O 2 EUR (t+2)).
 Proof.
   intros.
-  induction H; try subst; try contradiction.
-  
-
-
-Print exec_ctr_in_state_with_owner.
-
-
-Definition double_your_loan_ctr
-           (alice bob : Address)
-           (ctr_id dsc_id : Id)
-           (t0 : Time) :=
-  finctr ctr_id
-         dsc_id
-         (double_your_loan_desc t0)
-         alice
-         bob
-         bob
-         1.
-
-Ltac exec_double_your_loan H :=
-  match type of H with
-  | exec_ctr_in_state_with_owner (double_your_loan_ctr _ _ _ _ _) _ _ = Some _ =>
-    unfold double_your_loan_ctr, double_your_loan_desc, exec_ctr_in_state_with_owner in H; simpl in H; inversion H; clear H
-  end.
-
-
-Lemma bob_requests_double_loan_from_alice :
-  forall s1 alice bob ctr_id dsc_id result t0,
-    exec_ctr_in_state_with_owner
-      (double_your_loan_ctr alice bob ctr_id dsc_id t0) s1 bob =
-    Some result ->
-    exists ctr,
-      % ctr ∈ (res_contracts result) | alice --> bob | (Timebound t0 INF (Scale 2 (One EUR))) %.
-Proof.
+  induction H; intros.
+  - subst s2. omega.
+  - assert (S1 := H). assert (S2 := H7).
+    unfold is_executed in *.
+    apply steps_effect_over_contract with
+        (ctr := {|
+                 ctr_id := c_id;
+                 ctr_desc_id := dsc_id0;
+                 ctr_primitive := firl_description t;
+                 ctr_issuer := I;
+                 ctr_owner := O;
+                 ctr_proposed_owner := O;
+                 ctr_scale := 1 |}) in H; auto.
+    destruct H as [H | [H | H]].
+    + admit.
+Admitted.
